Update request_eval example by adding an operation case

examples/request_eval/new.dfy
@@ -14,8 +14,9 @@ module Types {
    // an atom consists of an operator that is applied to (the context value corresponding to) a key and a list values
    datatype Atom = | Atom(operation: Operation, key: string, values: seq<string>)
    // OneOf tests if the first context value with that key exists and is among the provided list of values
+   // AllOf tests if all context values with that key are among the provided list of values
    // Exists tests if any context entry with that key exists
-   datatype Operation = | OneOf | Exists
+   datatype Operation = | OneOf | AllOf | Exists
 }
 
 module Evaluation {
@@ -29,6 +30,7 @@ module Evaluation {
    function EvalAtom(ctx: Context, a: Atom): bool {
       match a.operation {
          case OneOf => EvalOneOf(ctx, a)
+         case AllOf => EvalAllOf(ctx, a)
          case Exists => EvalExists(ctx, a.key)
       }
    }
@@ -38,6 +40,10 @@ module Evaluation {
          case None() => false
          case Some(v) => v in a.values
       }
+   }
+
+   function EvalAllOf(ctx: Context, a: Atom): bool {
+      forall v:: v in LookupAll(ctx.entries, a.key) ==> v in a.values
    }
 
    function EvalExists(ctx: Context, k: string): bool {
@@ -50,5 +56,13 @@ module Evaluation {
          var e := entries[0];
          if e.key == k then Some(e.value)
          else Lookup(entries[1..], k)
+   }
+
+   function LookupAll(entries: seq<Entry>, k: string): seq<string> {
+      if entries == [] then []
+      else
+         var e := entries[0];
+         if e.key == k then [e.value] + LookupAll(entries[1..], k)
+         else LookupAll(entries[1..], k)
    }
 }
